defined structured footprint and prove eval_place_no_mem_error

rustfrontend/BorrowCheckSafe.v
@@ -253,46 +253,95 @@ Proof.
   lia.
 Qed.
 
+
 (** Test: try to define semantics well-typedness for a memory location *)
 
-Definition footprint := block -> Z -> Prop. 
+(* A tree structured footprint (maybe similar to some separation logic
+algebra) *)
+Inductive footprint : Type :=
+| fp_emp                        (* empty footprint *)
+| fp_box (b: block) (fp: footprint) (* A heap block storing values that occupy footprint fp *)
+| fp_struct (fpl: list footprint)
+| fp_enum (tag: Z) (fp: footprint)
+.
 
-Definition empty_footprint : footprint := fun b ofs => False.
 
-Definition footprint_equiv (fp1 fp2: footprint) :=
-  forall b ofs, fp1 b ofs <-> fp2 b ofs.
+Fixpoint footprint_flat (fp: footprint) : list block :=
+  match fp with
+  | fp_emp => nil
+  | fp_box b fp' =>
+      b :: footprint_flat fp'
+  | fp_struct fpl =>
+      concat (map footprint_flat fpl)
+  | fp_enum _ fp =>
+      footprint_flat fp
+  end.
 
-Definition footprint_incr (fp1 fp2: footprint) :=
-  forall b ofs, fp1 b ofs -> fp2 b ofs.
+Definition wf_footprint (fp: footprint) :=
+  list_norepet (footprint_flat fp).
 
-(** TODO: add some useful notations for footprint *)
-
-Definition remove_footprint (fp: footprint) b ofs sz :=
-  fun b1 ofs1 =>
-    ((b1 = b /\ ofs <= ofs1 < ofs + sz) -> False)
-    /\ fp b1 ofs1.
-
-Definition add_footprint (fp: footprint) b ofs sz :=
-  fun b1 ofs1 =>
-    ((b1 = b /\ ofs <= ofs1 < ofs + sz))
-    \/ fp b1 ofs1.
-
-Definition in_footprint (fp: footprint) b ofs sz :=
-  forall ofs1, ofs <= ofs1 < ofs + sz -> fp b ofs1.
-
-Definition merge_footprint (fp1 fp2: footprint) :=
-  fun b ofs => fp1 b ofs \/ fp2 b ofs.
-
-Definition merge_footprint_list (l: list footprint) :=
-  fun b ofs => exists fp, In fp l -> fp b ofs.
 
 Definition footprint_disjoint (fp1 fp2: footprint) :=
-  forall b ofs, fp1 b ofs -> fp2 b ofs -> False.
+  list_disjoint (footprint_flat fp1) (footprint_flat fp2).
 
-Definition footprint_disjoint_list (l: list footprint) :=
-  forall fp1 fp2, In fp1 l -> In fp2 l ->
-             ~ footprint_equiv fp1 fp2 ->
-             footprint_disjoint fp1 fp2.
+Inductive footprint_disjoint_list : list footprint -> Prop :=
+| fp_disjoint_nil: footprint_disjoint_list nil
+| fp_disjoint_cons: forall fp fpl,
+      list_disjoint (footprint_flat fp) (concat (map footprint_flat fpl)) ->
+      footprint_disjoint_list fpl ->
+      footprint_disjoint_list (fp::fpl)
+.
+
+Definition in_footprint (b: block) (fp: footprint) : Prop :=
+  In b (footprint_flat fp).
+
+(* Inductive footprint_path : Type := *)
+(* | fpp_leaf *)
+(* | fpp_box (p: footprint_path)        (* use p to select the box footprint *) *)
+(* | fpp_field (idx: Z) (p: footprint_path) (* select the nth field in struct footprint and use p to select the remaining *) *)
+(* | fpp_variant (tag: Z) (p: footprint_path) *)
+(* . *)
+  
+
+(* Footprint defined by property *)
+(* Definition footprint := block -> Z -> Prop.  *)
+
+(* Definition empty_footprint : footprint := fun b ofs => False. *)
+
+(* Definition footprint_equiv (fp1 fp2: footprint) := *)
+(*   forall b ofs, fp1 b ofs <-> fp2 b ofs. *)
+
+(* Definition footprint_incr (fp1 fp2: footprint) := *)
+(*   forall b ofs, fp1 b ofs -> fp2 b ofs. *)
+
+(* (** TODO: add some useful notations for footprint *) *)
+
+(* Definition remove_footprint (fp: footprint) b ofs sz := *)
+(*   fun b1 ofs1 => *)
+(*     ((b1 = b /\ ofs <= ofs1 < ofs + sz) -> False) *)
+(*     /\ fp b1 ofs1. *)
+
+(* Definition add_footprint (fp: footprint) b ofs sz := *)
+(*   fun b1 ofs1 => *)
+(*     ((b1 = b /\ ofs <= ofs1 < ofs + sz)) *)
+(*     \/ fp b1 ofs1. *)
+
+(* Definition in_footprint (fp: footprint) b ofs sz := *)
+(*   forall ofs1, ofs <= ofs1 < ofs + sz -> fp b ofs1. *)
+
+(* Definition merge_footprint (fp1 fp2: footprint) := *)
+(*   fun b ofs => fp1 b ofs \/ fp2 b ofs. *)
+
+(* Definition merge_footprint_list (l: list footprint) := *)
+(*   fun b ofs => exists fp, In fp l -> fp b ofs. *)
+
+(* Definition footprint_disjoint (fp1 fp2: footprint) := *)
+(*   forall b ofs, fp1 b ofs -> fp2 b ofs -> False. *)
+
+(* Definition footprint_disjoint_list (l: list footprint) := *)
+(*   forall fp1 fp2, In fp1 l -> In fp2 l -> *)
+(*              ~ footprint_equiv fp1 fp2 -> *)
+(*              footprint_disjoint fp1 fp2. *)
 
 Definition scalar_type (ty: type) : bool :=
   match ty with
@@ -308,89 +357,58 @@ Definition scalar_type (ty: type) : bool :=
 (* Semantics well typed location is mutually defined with semantics
 well typed value *)
 Inductive sem_wt_loc (ce: composite_env) (m: mem) : footprint -> block -> Z -> type -> Prop :=
-| sem_wt_box: forall ty b ofs fp
-    (INFP: in_footprint fp b ofs (size_chunk Mptr))
-    (* valid_access or range_perm ? *)
-    (VALID: Mem.range_perm m b ofs (ofs + size_chunk Mptr) Cur Freeable)
+| sem_wt_base: forall ty b ofs fp chunk
+    (MODE: Rusttypes.access_mode ty = Ctypes.By_value chunk)
     (WT: forall v,
-        Mem.load Mptr m b ofs = Some v ->
-        (* Box pointer must points to the start of a block *)
-        sem_wt_val ce m (remove_footprint fp b ofs (size_chunk Mptr)) v (Tbox ty)),
-    sem_wt_loc ce m fp b ofs (Tbox ty)
-| sem_wt_struct: forall fp b ofs co fpl orgs id
-    (CO: ce ! id = Some co)
-    (INFP: in_footprint fp b ofs (co_sizeof co))
-    (VALID: Mem.range_perm m b ofs (ofs + co_sizeof co) Cur Freeable)
-    (FPL: footprint_disjoint_list fpl)
-    (FPLCON: footprint_equiv fp (merge_footprint_list fpl))
+        Mem.load chunk m b ofs = Some v ->
+        sem_wt_val ce m fp v ty),
+    sem_wt_loc ce m fp b ofs ty
+| sem_wt_struct: forall b ofs co fpl orgs id
+    (CO: ce ! id = Some co)   
     (* all fields are semantically well typed *)
     (FWT: forall n fid fty ffp fofs,
         nth_error co.(co_members) n = Some (Member_plain fid fty) ->
         nth_error fpl n = Some ffp ->
         field_offset ce fid co.(co_members) = OK fofs ->
         sem_wt_loc ce m ffp b (ofs + fofs) fty),
-    sem_wt_loc ce m fp b ofs (Tstruct orgs id)
-| sem_wt_enum: forall fp b ofs orgs id co
-    (CO: ce ! id = Some co)
-    (INFP: in_footprint fp b ofs (co_sizeof co))
-    (VALID: Mem.range_perm m b ofs (ofs + co_sizeof co) Cur Freeable)
+    sem_wt_loc ce m (fp_struct fpl) b ofs (Tstruct orgs id)
+| sem_wt_enum: forall fp b ofs orgs id co tagz
+    (CO: ce ! id = Some co)    
     (* Interpret the field by the tag and prove that it is well-typed *)
-    (FWT: forall tag fid fty fofs,
-        Mem.load Mint32 m b ofs = Some (Vint tag) ->
-        list_nth_z co.(co_members) (Int.unsigned tag) = Some (Member_plain fid fty) ->
+    (TAG: Mem.load Mint32 m b ofs = Some (Vint (Int.repr tagz)))
+    (FWT: forall fid fty fofs,
+        list_nth_z co.(co_members) tagz = Some (Member_plain fid fty) ->
         variant_field_offset ce fid (co_members co) = OK fofs ->
-        sem_wt_loc ce m (remove_footprint fp b ofs fofs) b (ofs + fofs) fty),
-    sem_wt_loc ce m fp b ofs (Tvariant orgs id)
-(* | sem_wt_scalar: forall ty b ofs *)
-(*     (TY: scalar_type ty = true) *)
-(*     (VALID: Mem.range_perm m b ofs (ofs + sizeof ce ty) Cur Freeable) *)
-(*     (* To make sure that well-typed footprint is closed? *) *)
-(*     (WT: forall v chunk b' ofs', *)
-(*         Mem.load chunk m b ofs = Some v -> *)
-(*         v <> Vptr b' ofs'), *)
-(*     sem_wt_loc ce m (add_footprint empty_footprint b ofs (sizeof ce ty)) b ofs ty *)
+        sem_wt_loc ce m fp b (ofs + fofs) fty),
+    sem_wt_loc ce m (fp_enum tagz fp) b ofs (Tvariant orgs id)
 
 
 with sem_wt_val (ce: composite_env) (m: mem) : footprint -> val -> type -> Prop :=
 | wt_val_unit:
-  sem_wt_val ce m empty_footprint (Vint Int.zero) Tunit
+  sem_wt_val ce m fp_emp (Vint Int.zero) Tunit
 | wt_val_int: forall sz si n,
     Cop.cast_int_int sz si n = n ->
-    sem_wt_val ce m empty_footprint (Vint n) (Tint sz si)
+    sem_wt_val ce m fp_emp (Vint n) (Tint sz si)
 | wt_val_float: forall n,
-    sem_wt_val ce m empty_footprint (Vfloat n) (Tfloat Ctypes.F64)
+    sem_wt_val ce m fp_emp (Vfloat n) (Tfloat Ctypes.F64)
 | wt_val_single: forall n,
-    sem_wt_val ce m empty_footprint (Vsingle n) (Tfloat Ctypes.F32)
+    sem_wt_val ce m fp_emp (Vsingle n) (Tfloat Ctypes.F32)
 | wt_val_long: forall si n,
-    sem_wt_val ce m empty_footprint (Vlong n) (Tlong si)
-| wt_val_box: forall b ty fp,
+    sem_wt_val ce m fp_emp (Vlong n) (Tlong si)
+| wt_val_box: forall b ty fp
     (** Box pointer must be in the starting point of a block *)
-    sem_wt_loc ce m fp b 0 ty ->
-    sem_wt_val ce m fp (Vptr b Ptrofs.zero) (Tbox ty)
+    (* The value stored in (b,0) has type ty and occupies footprint fp *)
+    (WTLOC: sem_wt_loc ce m fp b 0 ty)
+    (VALID: Mem.range_perm m b 0 (sizeof ce ty) Cur Freeable),
+    sem_wt_val ce m (fp_box b fp) (Vptr b Ptrofs.zero) (Tbox ty)
 (* TODO *)
 (* | wt_val_ref: forall b ofs ty org mut, *)
 (*     sem_vt_val (Vptr b ofs) (Treference org mut ty) *)
-| wt_val_struct: forall id orgs b ofs fp co fpl
-    (CO: ce ! id = Some co)
-    (FPL: footprint_disjoint_list fpl)
-    (FPLCON: footprint_equiv fp (merge_footprint_list fpl))
-    (* Because struct value is passed by its address, we need to show
-    that all the fields in this address is well typed value *)
-    (FWT: forall n fid fty fofs v ffp,
-        nth_error co.(co_members) n = Some (Member_plain fid fty) ->
-        nth_error fpl n = Some ffp ->
-        field_offset ce fid co.(co_members) = OK fofs ->
-        deref_loc fty m b (Ptrofs.add ofs (Ptrofs.repr fofs)) v -> 
-        sem_wt_val ce m ffp v fty),
+| wt_val_struct: forall id orgs b ofs fp
+    (WTLOC: sem_wt_loc ce m fp b (Ptrofs.unsigned ofs) (Tstruct orgs id)),
     sem_wt_val ce m fp (Vptr b ofs) (Tstruct orgs id)
-| wt_val_enum: forall id orgs b ofs fp co
-    (CO: ce ! id = Some co)
-    (FWT: forall tag fid fty fofs v,
-        Mem.loadv Mint32 m (Vptr b ofs) = Some (Vint tag) ->
-        list_nth_z co.(co_members) (Int.unsigned tag) = Some (Member_plain fid fty) ->
-        variant_field_offset ce fid (co_members co) = OK fofs ->
-        deref_loc fty m b (Ptrofs.add ofs (Ptrofs.repr fofs)) v -> 
-        sem_wt_val ce m fp v fty),
+| wt_val_enum: forall id orgs b ofs fp
+    (WTLOC: sem_wt_loc ce m fp b (Ptrofs.unsigned ofs) (Tvariant orgs id)),
     sem_wt_val ce m fp (Vptr b ofs) (Tvariant orgs id)
 .
 
@@ -438,29 +456,31 @@ Canonical Structure li_rs :=
   |}.
 
 Inductive wt_rs_world :=
-  rsw (sg: rust_signature) (fp: footprint) (m: mem).
+  rsw (sg: rust_signature) (fpl: list footprint) (m: mem).
 
 Inductive wt_rs_query : wt_rs_world -> rust_query -> Prop :=
-| wt_rs_query_intro: forall sg fp m vf args fpl
-    (FPL: footprint_disjoint_list fpl)
-    (FPLCON: footprint_equiv fp (merge_footprint_list fpl))                       
+| wt_rs_query_intro: forall sg m vf args fpl
+    (DIS: footprint_disjoint_list fpl)
     (WT: sem_wt_val_list (sig_comp_env sg) m fpl args (sig_args sg)),
-    wt_rs_query (rsw sg fp m) (rsq vf sg args m)
+    wt_rs_query (rsw sg fpl m) (rsq vf sg args m)
 .
 
 (* Only consider ownership transfer for now. The footprints of generic
 origins are more complicated *)
 Inductive rsw_acc : wt_rs_world -> wt_rs_world -> Prop :=
-| rsw_acc_intro: forall sg fp fp' m m'
-    (UNC: Mem.unchanged_on (fun b ofs => ~ fp b ofs) m m')
-    (FPINCR: footprint_incr fp fp'),
-    rsw_acc (rsw sg fp m) (rsw sg fp' m').
+| rsw_acc_intro: forall sg fpl fpl' m m'
+    (UNC: Mem.unchanged_on (fun b ofs => Forall (fun fp => (~ in_footprint b fp)) fpl) m m'),
+    (** TODO: add footprint_list increase and some footprint separation properties  *)
+    (* (FPINCR: footprint_incr fp fp'), *)
+    rsw_acc (rsw sg fpl m) (rsw sg fpl' m').
 
 Inductive wt_rs_reply : wt_rs_world -> rust_reply -> Prop :=
-| wt_rs_reply_intro: forall rfp m rv sg fp
-    (WT: sem_wt_val (sig_comp_env sg) m rfp rv (sig_res sg))
-    (FPINCR: footprint_incr rfp fp),
-    wt_rs_reply (rsw sg fp m) (rsr rv m)
+| wt_rs_reply_intro: forall rfp m rv sg fpl
+    (WT: sem_wt_val (sig_comp_env sg) m rfp rv (sig_res sg)),
+    (** TODO: say that rfp is obtained from some footprint in the list
+    [fpl] *)
+    (* (FPINCR: footprint_incr rfp fp), *)
+    wt_rs_reply (rsw sg fpl m) (rsr rv m)
 .
 
 Definition wt_rs : invariant li_rs :=
@@ -515,111 +535,92 @@ from a stack block. *)
 
 Definition fp_map := PTree.t footprint.
 
-(** Definition of abstracter which maps a memory block to a place
-(i.e. the owner of this block) *)
-
-(* Definition mem_abstracter : Type := block -> Z -> option (place * Z). *)
-(* Why don't we use PTree? *)
-Definition mem_abstracter : Type := block -> option place.
-
-(** Extract footprint from abstracter *)
-
-Definition abs_footprint (abs: mem_abstracter) : footprint :=
-  fun b _ => match abs b with
-          | Some _ => True
-          | None => False
-          end.
-
-(* Two abstracters are disjoint if their footprints are disjoint *)
-Definition abs_disjoint (abs1 abs2: mem_abstracter) : Prop :=
-  footprint_disjoint (abs_footprint abs1) (abs_footprint abs2).
-
-Definition merge_abstracter (abs1 abs2: mem_abstracter) : mem_abstracter :=
-  fun b => match abs1 b, abs2 b with
-        | Some p, _ => Some p
-        | _, Some p => Some p
-        | None, None => None
-        end.
-
-Definition abs_equiv (abs1 abs2: mem_abstracter) : Prop :=
-  forall b, abs1 b = abs2 b.
-
 Section MATCH.
 
 Variable ce: composite_env.
-Variable abs: mem_abstracter.
 Variable fpm: fp_map.
 
-(* The footprint of a place *)
-Inductive place_footprint : place -> footprint -> Prop :=
-| place_footprint_deref: forall p p' fp ofs b ty
-    (FP: place_footprint p fp)
-    (ABS: abs b = Some p')
-    (SUBP: subplace ce p' p ofs),
-    place_footprint (Pderef p ty) (remove_footprint fp b ofs (sizeof ce (typeof_place p)))
-| place_footprint_field: forall p p' fp ofs b orgs id fid fty co fofs
-    (FP: place_footprint p fp)
-    (ABS: abs b = Some p')
-    (SUBP: subplace ce p' p ofs)
+(* The location and footprint of a place *)
+(* Fro place_footprint e p b ofs fp, it means that the location of [p]
+is (b, ofs) and the value stored in [p] occupies the footprint [fp] *)
+Inductive place_footprint (e: env) : place -> block -> Z -> footprint -> Prop :=
+| place_footprint_deref: forall p fp ofs1 b1 b2 ty
+    (* (b1, ofs1) *-> (b2, 0) *)
+    (FP: place_footprint e p b1 ofs1 (fp_box b2 fp)),
+    (* For now, we do not consider reference, so the location of *p is
+    always in the start of a block b2 *)
+    place_footprint e (Pderef p ty) b2 0 fp
+| place_footprint_field: forall p fp ofs b orgs id fid fty co fofs fpl tagz
+    (FP: place_footprint e p b ofs (fp_struct fpl))
     (TY: typeof_place p = Tstruct orgs id)
     (CO: ce!id = Some co)
-    (FOFS: field_offset ce id co.(co_members) = OK fofs),
-    (* fp - [(b,ofs), (b, ofs+sizeof(p))) + [(b,ofs+fofs), (b, ofs+fofs+sizeof(fty))) *)
-    place_footprint (Pfield p fid fty)
-    (add_footprint (remove_footprint fp b ofs (co_sizeof co)) b (ofs+fofs) (sizeof ce fty))
-| place_footprint_enum: forall p fp fid fty
-    (** FIXME: is it correct?  *)
-    (FP: place_footprint p fp),
-    place_footprint (Pdowncast p fid fty) fp
-| place_footprint_local: forall id fp ty
-    (FP: fpm ! id = Some fp),
-    place_footprint (Plocal id ty) fp
+    (FOFS: field_offset ce fid co.(co_members) = OK fofs)
+    (* find the location of fid to get the footprint *)
+    (TAG: field_tag fid co.(co_members) = Some tagz)
+    (FFP: list_nth_z fpl tagz = Some fp),
+    place_footprint e (Pfield p fid fty) b (ofs + fofs) fp
+| place_footprint_enum: forall p fp fid fty tagz b ofs orgs id co fofs
+    (FP: place_footprint e p b ofs (fp_enum tagz fp))
+    (TY: typeof_place p = Tvariant orgs id)
+    (CO: ce!id = Some co)
+    (FOFS: variant_field_offset ce fid co.(co_members) = OK fofs)
+    (TAGZ: list_nth_z co.(co_members) tagz = Some (Member_plain fid fty)),
+    place_footprint e (Pdowncast p fid fty) b (ofs + fofs) fp
+| place_footprint_local: forall id fp ty b
+    (FP: fpm ! id = Some fp)
+    (STK: e ! id = Some (b, ty)),
+    place_footprint e (Plocal id ty) b 0 fp
 .
 
 
-(* The value stored in m[b, ofs] is consistent with the type of p *)
-Inductive bmatch (m: mem) (b: block) (ofs: Z) (p: place) (own: own_env) : type -> Prop :=
-| bm_box: forall ty b1 ofs1
-    (* valid resource. If the loaded value is not a pointer, it is a
-    type error instead of a memory error *)
-    (* N.B. A compilcated situation is that [p] may fully own the
-    resource so that the all the blocks of the owned chain it points
-    to are not in the range of [own] environment. In this case, we
-    should show that the ownership chain is semantics well typed. But
-    if [p] just partially own the resoruce, we need to explicitly show
-    that the owner of the block it points to is [*p]. *)
-    (LOAD: Mem.load Mptr m b ofs = Some (Vptr b1 ofs1))
-    (VRES: 
+(* The value stored in m[b, ofs] is consistent with the type of p. [p]
+is owned. *)
+Inductive bmatch (m: mem) (b: block) (ofs: Z) (p: place) (own: own_env) : footprint -> type -> Prop :=
+| bm_box: forall ty b1 fp
+    (* valid resource. If the loaded value is not a pointer, it is a *)
+(*     type error instead of a memory error *)
+    (* N.B. A compilcated situation is that [p] may fully own the *)
+(*     resource so that the all the blocks of the owned chain it points *)
+(*     to are not in the range of [own] environment. In this case, we *)
+(*     should show that the ownership chain is semantics well typed. But *)
+(*     if [p] just partially own the resoruce, we need to explicitly show *)
+(*     that the owner of the block it points to is [*p]. *)
+    (LOAD: Mem.load Mptr m b ofs = Some (Vptr b1 Ptrofs.zero))
+    (VRES:
         (** Case1: p is partially owned *)
-        (* p owns the location it points to. Box pointer must points
-        to the start of a block and *p is the owner of this block *)
-        (is_shallow_owned own p = true -> (ofs1 = Ptrofs.zero /\ abs b1 = Some (Pderef p ty)))
-        (** Case2: p is fully owned: own b1 is None. How to get the
-        footprint of this semantics well typedness? *)
-        /\ (is_deep_owned own p = true ->
-           (exists fp, place_footprint p fp
-                  /\ sem_wt_loc ce m fp b ofs (typeof_place p)))),
-    bmatch m b ofs p own (Tbox ty)
-| bm_struct: forall orgs id
-    (* all fields in the struct satisfy bmatch *)
-    (FMATCH: forall co fid fty fofs,
-        ce ! id = Some co ->
-        In (Member_plain fid fty) co.(co_members) ->       
+        (* p owns the location it points to. Box pointer must points *)
+(*         to the start of a block and *p is the owner of this block *)
+        (* (is_shallow_owned own p = true -> (ofs1 = Ptrofs.zero /\ abs b1 = Some (Pderef p ty))) *)
+        (** Case2: p is fully owned: own b1 is None. How to get the *)
+        (* footprint of this semantics well typedness? *)
+        (* /\ (is_deep_owned own p = true -> *)
+        (*    (exists fp, place_footprint p fp *)
+      (*         /\ sem_wt_loc ce m fp b ofs (typeof_place p)))), *)
+      Mem.range_perm m b1 0 (sizeof ce ty) Cur Freeable),
+    bmatch m b ofs p own (fp_box b1 fp) (Tbox ty)
+| bm_struct: forall co fpl orgs id
+    (CO: ce ! id = Some co)
+    (* all fields are semantically well typed *)
+    (FMATCH: forall n fid fty ffp fofs,
+        nth_error co.(co_members) n = Some (Member_plain fid fty) ->
+        nth_error fpl n = Some ffp ->
         field_offset ce fid co.(co_members) = OK fofs ->
-        bmatch m b (ofs + fofs) (Pfield p fid fty) own fty),
-    bmatch m b ofs p own (Tstruct orgs id)
-| bm_enum: forall orgs id
-    (FMATCH: forall co fid fty fofs tag,
-        ce ! id = Some co ->
-        (* load tag *)
-        Mem.load Mint32 m b ofs = Some (Vint tag) ->
-        list_nth_z co.(co_members) (Int.unsigned tag) = Some (Member_plain fid fty) ->
-        variant_field_offset ce fid (co_members co) = OK fofs ->        
-        bmatch m b (ofs + fofs) (Pdowncast p fid fty) own fty),
-    bmatch m b ofs p own (Tvariant orgs id)
+        bmatch m b (ofs + fofs) (Pfield p fid fty) own ffp fty),
+    bmatch m b ofs p own (fp_struct fpl) (Tstruct orgs id)
+| bm_enum: forall fp orgs id co tagz
+    (CO: ce ! id = Some co)
+    (* Interpret the field by the tag and prove that it is well-typed *)
+    (* [p] whose value has footprint (fp_enum tagz fp) is actually has
+    tag tagz *)
+    (TAG: Mem.load Mint32 m b ofs = Some (Vint (Int.repr tagz))) 
+    (FMATCH: forall fid fty fofs,        
+        list_nth_z co.(co_members) tagz = Some (Member_plain fid fty) ->
+        variant_field_offset ce fid (co_members co) = OK fofs ->
+        bmatch m b (ofs + fofs) (Pdowncast p fid fty) own fp fty),
+    bmatch m b ofs p own (fp_enum tagz fp) (Tvariant orgs id)
 | bm_scalar: forall ty,
     scalar_type ty = true ->
-    bmatch m b ofs p own ty
+    bmatch m b ofs p own fp_emp ty
 (** TODO: bm_reference  *)
 .
 
@@ -627,29 +628,31 @@ Inductive bmatch (m: mem) (b: block) (ofs: Z) (p: place) (own: own_env) : type -
 
 (* bmatch under subplace *)
 
-Lemma bmatch_subplace: forall p p' ofs ofs' own m b,
-    bmatch m b ofs p own (typeof_place p) ->
-    subplace ce p p' ofs' ->
-    bmatch m b (ofs + ofs') p' own (typeof_place p').
-Admitted.
+(* Lemma bmatch_subplace: forall p p' ofs ofs' own m b, *)
+(*     bmatch m b ofs p own (typeof_place p) -> *)
+(*     subplace ce p p' ofs' -> *)
+(*     bmatch m b (ofs + ofs') p' own (typeof_place p'). *)
+(* Admitted. *)
 
 (** TODO: support alias analysis domain *)
-Definition mmatch (m: mem) (own: own_env) : Prop :=
-  forall b p,
-    abs b = Some p ->
-    (Mem.range_perm m b 0 (sizeof ce (typeof_place p)) Cur Freeable
-    /\ bmatch m b 0 p own (typeof_place p)).
+Definition mmatch (m: mem) (e: env) (own: own_env) : Prop :=
+  forall p b ofs fp,
+    place_footprint e p b ofs fp ->
+    (* We only consider the initialized place *)
+    is_owned own p = true ->
+    bmatch m b ofs p own fp (typeof_place p).
+    
+    
+(* Record wf_footprint (e: env) : Prop := *)
+(*   { wf_local_env: forall id b ty, *)
+(*       e ! id = Some (b, ty) -> *)
+(*       abs b = Some (Plocal id ty); *)
 
-Record wf_abs (e: env) : Prop :=
-  { wf_local_env: forall id b ty,
-      e ! id = Some (b, ty) ->
-      abs b = Some (Plocal id ty);
-
-    (* all mapped places are in the range of Ptrofs.max_unsigned *)
-    wf_place_size: forall b p,
-      abs b = Some p ->
-      sizeof ce (typeof_place p) < Ptrofs.max_unsigned
-  }.
+(*     (* all mapped places are in the range of Ptrofs.max_unsigned *) *)
+(*     wf_place_size: forall b p, *)
+(*       abs b = Some p -> *)
+(*       sizeof ce (typeof_place p) < Ptrofs.max_unsigned *)
+(*   }. *)
 
 End MATCH.
 
@@ -675,6 +678,7 @@ Proof.
   induction p; simpl; auto.
   congruence.
   intros. inv H. auto.
+  intros. inv H. auto.
 Qed.
 
 Lemma place_dominator_strict_prefix: forall p p',
@@ -686,8 +690,8 @@ Proof.
     unfold is_prefix_strict. simpl. destruct (place_eq p p). auto. congruence.
   - inv H.
     unfold is_prefix_strict. simpl. destruct (place_eq p' p'). auto. congruence.
-  - exploit IHp. eauto. intros A. eapply is_prefix_strict_trans. eauto.
-    unfold is_prefix_strict. simpl. destruct (place_eq p p). auto. congruence.
+  - inv H.
+    unfold is_prefix_strict. simpl. destruct (place_eq p' p'). auto. congruence.
 Qed.
 
 Lemma dominator_of_shallow_owned_place: forall own p,
@@ -736,148 +740,145 @@ Let ce := ge.(genv_cenv).
 Hypothesis CONSISTENT: composite_env_consistent ce.
 
 Inductive sound_state: state -> Prop :=
-| sound_regular_state: forall f s k e own m entry cfg pc instr ae Σ Γ Δ abs fpm
+| sound_regular_state: forall f s k e own m entry cfg pc instr ae Σ Γ Δ fpm
     (CFG: generate_cfg f.(fn_body) = OK (entry, cfg))
     (INSTR: cfg ! pc = Some instr)
     (MSTMT: match_instr_stmt f.(fn_body) instr s k)
     (CHK: borrow_check ce f = OK ae)
     (AS: ae ! pc = Some (AE.State Σ Γ Δ))
-    (MM: mmatch ce abs fpm m own)
-    (WF: wf_abs ce abs e),
+    (MM: mmatch ce fpm m e own),
     sound_state (State f s k e own m)
 .
 
 
 (** The address of a place is consistent with the abstracter. For now,
 we do not consider reference *)
-Lemma eval_place_sound: forall e m p b ofs abs own fpm
+Lemma eval_place_sound: forall e m p b ofs own fpm
     (EVAL: eval_place ce e m p b ofs)
-    (MM: mmatch ce abs fpm m own)
-    (WFABS: wf_abs ce abs e)
+    (MM: mmatch ce fpm m e own)
     (WFOWN: wf_own_env own)
     (WT: wt_place (env_to_tenv e) ce p)
     (* evaluating the address of p does not require that p is
     owned. Shallow own is used in bmatch *)
-    (POWN: place_dominator_shallow_own own p = true),
-  exists p', abs b = Some p'
-        /\ subplace ce p' p (Ptrofs.unsigned ofs)
+    (POWN: place_dominator_own own p = true),
+  (* Do we need to specify the properties of fp? Do we need to show
+  the permission of the location of p? *)
+    exists fp, place_footprint ce fpm e p b (Ptrofs.unsigned ofs) fp.
     (* if consider reference, we cannot say that p is a subplace of
     p', instead we need to state that the owner p points to is a
     subplace of p' *)
-.
-Proof.
-  induction 1; intros.
-  (* Plocal *)
-  - rewrite Ptrofs.unsigned_zero.
-    exists (Plocal id ty). split.
-    eapply wf_local_env; eauto.
-    econstructor.
-  (* Pfield *)
-  - inv WT.
-    eapply place_dominator_shallow_own_shallow_prefix with (p':= p) in POWN.
-    exploit IHEVAL. 1-5: auto.
-    intros (p' & ABS & SUBP).
-    exists p'. split. auto.
-    (* two type facts, reduce one *)
-    rewrite H in H6. inv H6. rewrite H0 in H7. inv H7.
-    (* *** Begin range proof *** *)
-    (* Can we require that the size of p' is in the range of
-    Ptrofs.max_unsigned, so that any subplace is in this range
-    (including its successor) *)
-    exploit wf_place_size; eauto. intros PSIZE.
-    generalize (subplace_upper_bound _ _ _ _ _ SUBP CONSISTENT H5 (Z.lt_le_incl _ _ PSIZE)).    rewrite H. simpl. rewrite H0.
-    erewrite co_consistent_sizeof; eauto. rewrite H9. simpl.
-    assert (ALPOS: co_alignof co0 > 0).
-    { exploit co_alignof_two_p. intros (n & ALPOW).
-      rewrite ALPOW. rewrite two_power_nat_equiv.
-      generalize (Nat2Z.is_nonneg n). intros A.
-      exploit Z.pow_pos_nonneg. instantiate (1:= 2). lia.
-      eauto. lia. }
-    generalize (align_le (sizeof_struct ce (co_members co0)) _ ALPOS).
-    intros STRUCTSZ BOUND.
-    exploit field_offset_in_range; eauto. intros (RANGE1 & RANGE2).
-    generalize (Ptrofs.unsigned_range ofs). intros OFSRANGE.
-    generalize (sizeof_pos ce ty). intros TYSZPOS.
-    (* *** End range proof *** *)
-    rewrite Ptrofs.add_unsigned.
-    do 2 rewrite Ptrofs.unsigned_repr.
-    econstructor. auto. eauto. eauto.
-    eauto.
-    (** dirty work: specify the requirement to prevent overflow *)
-    lia. lia. lia.
-    unfold is_shallow_prefix. eapply orb_true_intro.
-    right. simpl. destruct (place_eq p p). auto. congruence.    
-  (* Pdowncast *)
-  - inv WT.
-    eapply place_dominator_shallow_own_shallow_prefix with (p':= p) in POWN.
-    exploit IHEVAL. 1-5: auto.
-    intros (p' & ABS & SUBP).
-    exists p'. split. auto.
-    (* two type facts, reduce one *)
-    rewrite H in H8. inv H8. rewrite H0 in H9. inv H9.
-    (* *** Begin range proof *** *)
-    exploit wf_place_size; eauto. intros PSIZE.
-    generalize (subplace_upper_bound _ _ _ _ _ SUBP CONSISTENT H7 (Z.lt_le_incl _ _ PSIZE)).    rewrite H. simpl. rewrite H0.
-    erewrite co_consistent_sizeof; eauto. rewrite H11. simpl.
-    assert (ALPOS: co_alignof co0 > 0).
-    { exploit co_alignof_two_p. intros (n & ALPOW).
-      rewrite ALPOW. rewrite two_power_nat_equiv.
-      generalize (Nat2Z.is_nonneg n). intros A.
-      exploit Z.pow_pos_nonneg. instantiate (1:= 2). lia.
-      eauto. lia. }
-    generalize (align_le (sizeof_variant ce (co_members co0)) _ ALPOS).
-    intros ENUMSZ BOUND.
-    exploit variant_field_offset_in_range; eauto. intros (RANGE1 & RANGE2).
-    generalize (Ptrofs.unsigned_range ofs). intros OFSRANGE.
-    generalize (sizeof_pos ce ty). intros TYSZPOS.
-    (* *** End range proof *** *)
-    rewrite Ptrofs.add_unsigned.
-    do 2 rewrite Ptrofs.unsigned_repr.
-    econstructor. auto. eauto. eauto.
-    eauto.
-    (** dirty work: specify the requirement to prevent overflow *)
-    lia. lia. lia.
-    (* shallow prefix *)
-    unfold is_shallow_prefix. eapply orb_true_intro.
-    right. simpl. destruct (place_eq p p). auto. congruence.
-  (* Pderef *)
-  - inv WT.
-    exploit IHEVAL. eauto. eauto. eauto. eauto.
-    (* place dominator is shallow owned *)
-    unfold place_dominator_shallow_own in POWN. simpl in POWN.
-    eapply dominator_of_shallow_owned_place. auto. auto.
-    intros (p' & ABS & SUBP).
-    eapply MM in ABS. destruct ABS as (A & B).
-    (* p is a subplace of p' and p' bmatch implies p bmatch *)
-    exploit bmatch_subplace; eauto. rewrite Z.add_0_l. intros BM.
-    (* typeof_place p must be box/reference *)
-    destruct (typeof_place p) eqn: TYP; simpl in *; try congruence.
-    (* Tbox *)
-    + inv BM.
-      (* deref_loc and LOAD in sem_wt_loc say the same thing *)
-      inv H; simpl in *; try congruence. inv H0. rewrite LOAD in H1. inv H1.
-      inv H3.
-      (* Now we need to say that p is shallow owned *)
-      unfold place_dominator_shallow_own in POWN. simpl in POWN.
-      destruct VRES as (C & D).
-      eapply C in POWN. destruct POWN as (E & F). subst.
-      exists (Pderef p ty). split. auto.
-      rewrite Ptrofs.unsigned_zero. constructor.
-      (* box is not scalar type *)
-      simpl in H0. congruence.
-    (* reference *)
-    + admit.
+(* Proof. *)
+(*   induction 1; intros. *)
+(*   (* Plocal *) *)
+(*   - rewrite Ptrofs.unsigned_zero. *)
+(*     exists (Plocal id ty). split. *)
+(*     eapply wf_local_env; eauto. *)
+(*     econstructor. *)
+(*   (* Pfield *) *)
+(*   - inv WT. *)
+(*     eapply place_dominator_shallow_own_shallow_prefix with (p':= p) in POWN. *)
+(*     exploit IHEVAL. 1-5: auto. *)
+(*     intros (p' & ABS & SUBP). *)
+(*     exists p'. split. auto. *)
+(*     (* two type facts, reduce one *) *)
+(*     rewrite H in H6. inv H6. rewrite H0 in H7. inv H7. *)
+(*     (* *** Begin range proof *** *) *)
+(*     (* Can we require that the size of p' is in the range of *)
+(*     Ptrofs.max_unsigned, so that any subplace is in this range *)
+(*     (including its successor) *) *)
+(*     exploit wf_place_size; eauto. intros PSIZE. *)
+(*     generalize (subplace_upper_bound _ _ _ _ _ SUBP CONSISTENT H5 (Z.lt_le_incl _ _ PSIZE)).    rewrite H. simpl. rewrite H0. *)
+(*     erewrite co_consistent_sizeof; eauto. rewrite H9. simpl. *)
+(*     assert (ALPOS: co_alignof co0 > 0). *)
+(*     { exploit co_alignof_two_p. intros (n & ALPOW). *)
+(*       rewrite ALPOW. rewrite two_power_nat_equiv. *)
+(*       generalize (Nat2Z.is_nonneg n). intros A. *)
+(*       exploit Z.pow_pos_nonneg. instantiate (1:= 2). lia. *)
+(*       eauto. lia. } *)
+(*     generalize (align_le (sizeof_struct ce (co_members co0)) _ ALPOS). *)
+(*     intros STRUCTSZ BOUND. *)
+(*     exploit field_offset_in_range; eauto. intros (RANGE1 & RANGE2). *)
+(*     generalize (Ptrofs.unsigned_range ofs). intros OFSRANGE. *)
+(*     generalize (sizeof_pos ce ty). intros TYSZPOS. *)
+(*     (* *** End range proof *** *) *)
+(*     rewrite Ptrofs.add_unsigned. *)
+(*     do 2 rewrite Ptrofs.unsigned_repr. *)
+(*     econstructor. auto. eauto. eauto. *)
+(*     eauto. *)
+(*     (** dirty work: specify the requirement to prevent overflow *) *)
+(*     lia. lia. lia. *)
+(*     unfold is_shallow_prefix. eapply orb_true_intro. *)
+(*     right. simpl. destruct (place_eq p p). auto. congruence.     *)
+(*   (* Pdowncast *) *)
+(*   - inv WT. *)
+(*     eapply place_dominator_shallow_own_shallow_prefix with (p':= p) in POWN. *)
+(*     exploit IHEVAL. 1-5: auto. *)
+(*     intros (p' & ABS & SUBP). *)
+(*     exists p'. split. auto. *)
+(*     (* two type facts, reduce one *) *)
+(*     rewrite H in H8. inv H8. rewrite H0 in H9. inv H9. *)
+(*     (* *** Begin range proof *** *) *)
+(*     exploit wf_place_size; eauto. intros PSIZE. *)
+(*     generalize (subplace_upper_bound _ _ _ _ _ SUBP CONSISTENT H7 (Z.lt_le_incl _ _ PSIZE)).    rewrite H. simpl. rewrite H0. *)
+(*     erewrite co_consistent_sizeof; eauto. rewrite H11. simpl. *)
+(*     assert (ALPOS: co_alignof co0 > 0). *)
+(*     { exploit co_alignof_two_p. intros (n & ALPOW). *)
+(*       rewrite ALPOW. rewrite two_power_nat_equiv. *)
+(*       generalize (Nat2Z.is_nonneg n). intros A. *)
+(*       exploit Z.pow_pos_nonneg. instantiate (1:= 2). lia. *)
+(*       eauto. lia. } *)
+(*     generalize (align_le (sizeof_variant ce (co_members co0)) _ ALPOS). *)
+(*     intros ENUMSZ BOUND. *)
+(*     exploit variant_field_offset_in_range; eauto. intros (RANGE1 & RANGE2). *)
+(*     generalize (Ptrofs.unsigned_range ofs). intros OFSRANGE. *)
+(*     generalize (sizeof_pos ce ty). intros TYSZPOS. *)
+(*     (* *** End range proof *** *) *)
+(*     rewrite Ptrofs.add_unsigned. *)
+(*     do 2 rewrite Ptrofs.unsigned_repr. *)
+(*     econstructor. auto. eauto. eauto. *)
+(*     eauto. *)
+(*     (** dirty work: specify the requirement to prevent overflow *) *)
+(*     lia. lia. lia. *)
+(*     (* shallow prefix *) *)
+(*     unfold is_shallow_prefix. eapply orb_true_intro. *)
+(*     right. simpl. destruct (place_eq p p). auto. congruence. *)
+(*   (* Pderef *) *)
+(*   - inv WT. *)
+(*     exploit IHEVAL. eauto. eauto. eauto. eauto. *)
+(*     (* place dominator is shallow owned *) *)
+(*     unfold place_dominator_shallow_own in POWN. simpl in POWN. *)
+(*     eapply dominator_of_shallow_owned_place. auto. auto. *)
+(*     intros (p' & ABS & SUBP). *)
+(*     eapply MM in ABS. destruct ABS as (A & B). *)
+(*     (* p is a subplace of p' and p' bmatch implies p bmatch *) *)
+(*     exploit bmatch_subplace; eauto. rewrite Z.add_0_l. intros BM. *)
+(*     (* typeof_place p must be box/reference *) *)
+(*     destruct (typeof_place p) eqn: TYP; simpl in *; try congruence. *)
+(*     (* Tbox *) *)
+(*     + inv BM. *)
+(*       (* deref_loc and LOAD in sem_wt_loc say the same thing *) *)
+(*       inv H; simpl in *; try congruence. inv H0. rewrite LOAD in H1. inv H1. *)
+(*       inv H3. *)
+(*       (* Now we need to say that p is shallow owned *) *)
+(*       unfold place_dominator_shallow_own in POWN. simpl in POWN. *)
+(*       destruct VRES as (C & D). *)
+(*       eapply C in POWN. destruct POWN as (E & F). subst. *)
+(*       exists (Pderef p ty). split. auto. *)
+(*       rewrite Ptrofs.unsigned_zero. constructor. *)
+(*       (* box is not scalar type *) *)
+(*       simpl in H0. congruence. *)
+(*     (* reference *) *)
+(*     + admit. *)
 Admitted.
 
 
-Lemma eval_place_no_mem_error: forall e m p abs own fpm
-    (MM: mmatch ce abs fpm m own)
-    (WFABS: wf_abs ce abs e)
+Lemma eval_place_no_mem_error: forall e m p own fpm
+    (MM: mmatch ce fpm m e own)
     (WFOWN: wf_own_env own)
     (WT: wt_place (env_to_tenv e) ce p)
     (* evaluating the address of p does not require that p is
     owned. Shallow own is used in bmatch *)
-    (POWN: place_dominator_shallow_own own p = true)
+    (POWN: place_dominator_own own p = true)
     (ERR: eval_place_mem_error ce e m p),
     False.
 Proof.
@@ -890,91 +891,94 @@ Proof.
   (* Pderef *)
   - inv ERR.
     (* eval p error *)
-    + eapply IHp. 1-4: eauto.
+    + eapply IHp. 1-3: eauto.
       inv WT. auto.
-      eapply dominator_of_shallow_owned_place. auto. auto.
+      eapply wf_own_dominator. auto. auto.
       auto.
     (* deref error *)
     + inv WT.
-      exploit eval_place_sound. 1-5: eauto.
-      eapply dominator_of_shallow_owned_place. auto.
-      unfold place_dominator_shallow_own in POWN. simpl in POWN.
-      auto.
-      intros (p' & ABS & SUBP).
-      (* The block of p' is valid block *)
-      eapply MM in ABS. destruct ABS as (PERM & BM).
-      (* inv deref_loc_error *)
-      inv H2. eapply H0.
-      (** Show that location of p is valid_access *)
-      red. split.
-      * (* prove the location of p is in the range of p' *)
-        eapply Mem.range_perm_implies with (p1:= Freeable).
-        red. intros. eapply PERM.
-        exploit subplace_in_range; eauto.
-        erewrite <- sizeof_by_value; eauto.
-        lia.
-        constructor.
-      * exploit subplace_align; eauto.
-        intros AL.
-        eapply Z.divide_trans. eapply alignof_by_value. eauto.
-        eauto.
+      (* p is owned *)
+      assert (OWN: is_owned own p = true) by auto.
+      exploit eval_place_sound. 1-4: eauto.
+      eapply wf_own_dominator; auto.
+      intros (fp & PFP).
+      exploit MM; eauto.
+      intros BM. inv H2. apply H0.
+      (* case analysis of the p type *)
+      destruct (typeof_place p); simpl in H4; try congruence.
+      (* Box type *)
+      * simpl in H. inv H. inv BM.
+        eapply Mem.load_valid_access; eauto.
+        simpl in H. congruence.
+      (* reference type *)
+      * admit.
   (* Pdowncast *)
   - inv ERR.
     (* eval_place p error *)
-    + eapply IHp; eauto.
+    + eapply IHp. 1-3: eauto.
       inv WT. auto.
+      eapply wf_own_dominator; eauto.
+      auto.
     (* load tag error *)
     + inv WT.
-      exploit eval_place_sound. 1-5: eauto.
-      eapply place_dominator_shallow_own_shallow_prefix. eauto.
-      unfold is_shallow_prefix. simpl. destruct (place_eq p p); try congruence.
-      simpl. eapply orb_true_r.
-      intros (p' & ABS & SUBP).
-      (* The block of p' is valid block *)
-      eapply MM in ABS. destruct ABS as (PERM & BM).
-      (* show that the location of tag is valid *)
-      eapply H3.
-      red. split.
-      * eapply Mem.range_perm_implies with (p1:= Freeable).
-        red. intros. eapply PERM.
-        exploit subplace_in_range; eauto.
-        assert (SZTAGLE: size_chunk Mint32 <= sizeof ce (typeof_place p)).
-        { rewrite H5. simpl.
-          rewrite H6. erewrite co_consistent_sizeof; eauto.
-          rewrite H8. simpl.
-          generalize (sizeof_variant_ge4 ce (co_members co)). intros A.
-          assert (ALGE: co_alignof co > 0).
-          { exploit co_alignof_two_p. intros (n & COAL).
-            rewrite COAL. apply two_power_nat_pos. }
-          generalize (align_le (sizeof_variant ce (co_members co)) _ ALGE).
-          lia. }
-        lia.
-        constructor.
-      * exploit subplace_align; eauto.
-        assert (AL: (align_chunk Mint32 | alignof ce (typeof_place p))).
-        { rewrite H5. simpl.
-          rewrite H6. erewrite co_consistent_alignof; eauto.
-          rewrite H8. simpl.
-          (* easy but tedious *)
-          exploit alignof_composite_two_p'.
-          intros (n & AL). erewrite AL.
-          rewrite two_power_nat_equiv.
-          replace 4 with (2 ^ 2) by lia.
-          unfold Z.max.
-          destruct (2 ^ 2 ?= (2 ^ Z.of_nat n)) eqn:  LE.
-          eapply Z.divide_refl.
-          (* case 2^2 < 2 ^ n *)
-          eapply Z.pow_lt_mono_r_iff in LE.
-          exploit Z.le_exists_sub. eapply Z.lt_le_incl.
-          eauto. intros (p0 & PEQ & PLE). rewrite PEQ.
-          rewrite Z.pow_add_r. eapply Z.divide_factor_r.
-          auto. lia. lia.
-          eapply Nat2Z.is_nonneg.
-          eapply Z.divide_refl. }
-        intros ALTY.
-        eapply Z.divide_trans. eauto.
-        eauto.
-Qed.
+      assert (OWN: is_owned own p = true) by auto.
+      exploit eval_place_sound. 1-4: eauto.
+      eapply wf_own_dominator; eauto.
+      intros (fp & PFP).
+      exploit MM; eauto. rewrite H5. intros BM.
+      inv BM.
+      eapply H3. eapply Mem.load_valid_access; eauto.
+      simpl in H. congruence.
+      (* auto. *)
+      (* eapply place_dominator_shallow_own_shallow_prefix. eauto. *)
+      (* unfold is_shallow_prefix. simpl. destruct (place_eq p p); try congruence. *)
+      (* simpl. eapply orb_true_r. *)
+      (* intros (p' & ABS & SUBP). *)
+      (* (* The block of p' is valid block *) *)
+      (* eapply MM in ABS. destruct ABS as (PERM & BM). *)
+      (* (* show that the location of tag is valid *) *)
+      (* eapply H3. *)
+      (* red. split. *)
+      (* * eapply Mem.range_perm_implies with (p1:= Freeable). *)
+      (*   red. intros. eapply PERM. *)
+      (*   exploit subplace_in_range; eauto. *)
+      (*   assert (SZTAGLE: size_chunk Mint32 <= sizeof ce (typeof_place p)). *)
+      (*   { rewrite H5. simpl. *)
+      (*     rewrite H6. erewrite co_consistent_sizeof; eauto. *)
+      (*     rewrite H8. simpl. *)
+      (*     generalize (sizeof_variant_ge4 ce (co_members co)). intros A. *)
+      (*     assert (ALGE: co_alignof co > 0). *)
+      (*     { exploit co_alignof_two_p. intros (n & COAL). *)
+      (*       rewrite COAL. apply two_power_nat_pos. } *)
+      (*     generalize (align_le (sizeof_variant ce (co_members co)) _ ALGE). *)
+      (*     lia. } *)
+      (*   lia. *)
+      (*   constructor. *)
+      (* * exploit subplace_align; eauto. *)
+      (*   assert (AL: (align_chunk Mint32 | alignof ce (typeof_place p))). *)
+      (*   { rewrite H5. simpl. *)
+      (*     rewrite H6. erewrite co_consistent_alignof; eauto. *)
+      (*     rewrite H8. simpl. *)
+      (*     (* easy but tedious *) *)
+      (*     exploit alignof_composite_two_p'. *)
+      (*     intros (n & AL). erewrite AL. *)
+      (*     rewrite two_power_nat_equiv. *)
+      (*     replace 4 with (2 ^ 2) by lia. *)
+      (*     unfold Z.max. *)
+      (*     destruct (2 ^ 2 ?= (2 ^ Z.of_nat n)) eqn:  LE. *)
+      (*     eapply Z.divide_refl. *)
+      (*     (* case 2^2 < 2 ^ n *) *)
+      (*     eapply Z.pow_lt_mono_r_iff in LE. *)
+      (*     exploit Z.le_exists_sub. eapply Z.lt_le_incl. *)
+      (*     eauto. intros (p0 & PEQ & PLE). rewrite PEQ. *)
+      (*     rewrite Z.pow_add_r. eapply Z.divide_factor_r. *)
+      (*     auto. lia. lia. *)
+      (*     eapply Nat2Z.is_nonneg. *)
+      (*     eapply Z.divide_refl. } *)
+      (*   intros ALTY. *)
+      (*   eapply Z.divide_trans. eauto. *)
+      (*   eauto. *)
+Admitted.
 
 
 
